feat: complete csubst lemma for LBT

theories/Semantics.v
@@ -7,8 +7,10 @@ From MetaCoq.Utils Require Import utils.
 From VTL Require Import PIR BigStepPIR Subset Translation Utils.
 
 Existing Instance EWcbvEval.default_wcbv_flags.
+Set Default Goal Selector "!".
 
 Import Coq.Strings.String.
+Import Coq.Logic.Eqdep.
 Import MCMonadNotation.
 
 Notation "t' '⇓ₚ' v'" :=
@@ -16,110 +18,206 @@ Notation "t' '⇓ₚ' v'" :=
   (at level 50).
 
 Ltac solve_pir_eval := split; [(eexists ; eauto using eval) | constructor].
-Ltac tl_reflect  Htl  := apply translate_reflect in Htl  as ?tlt.
-Ltac tlt_reflect Htlt := apply translate_reflect in Htlt as ?tl.
+Ltac tl_reflect Htl := apply translate_reflect in Htl as ?tlt.
 Ltac invs H := inversion H; subst.
 
 Definition gal_id :=
   tLambda (BasicAst.nNamed "x"%bs) (tRel 0).
 
-(* To be infered from lambda binders *)
-Lemma fresh_axiom : forall (Γ : list bs) x s,
-  ~ (In x Γ) ->
-  ~ (In x (s :: Γ)).
-Admitted.
-
 Lemma weaken_ctx : forall Γ x t ann t',
-  ~ (In x Γ) ->
-  InSubset Γ t ->
-  translate_term remap_env Γ t ann = Some t' ->
-  translate_term remap_env (Γ ++ [x]) t ann = Some t'.
+  translatesTo remap_env Γ t ann t' ->
+  translatesTo remap_env (Γ ++ [x]) t ann t'.
 Proof.
-  intros Γ x t ann t'' nIn sub. revert t''.
-  induction sub; intros t' tl_t;
-  tl_reflect tl_t; inversion tlt.
-  - auto.
-  - simpl. apply nth_error_Some_length in H.
-    rewrite nth_error_app1, H2. auto. apply H.
-  - (* lambda case *) admit.
-  - (* app *) admit.
-Admitted.
-
-Lemma tl_closed : forall Γ t ann t',
-  InSubset Γ t ->
-  translate_term remap_env Γ t ann = Some t' ->
-    closedn #|Γ| t /\ 
-    closedUnder (map String.to_string Γ) t'.
-Proof.
-  intros Γ t ann t'' sub. revert t''. 
-  induction sub; intros t' tl_t; tl_reflect tl_t.
-  - inversion tlt. auto. 
-  - split.
-    + now apply nth_error_Some_length, Nat.ltb_lt in H.
-    + inversion tlt. simpl. apply nth_error_In in H2.
-      apply existsb_exists. exists (bs_to_s x). 
-      split.
-      * apply in_map. apply H2.
-      * now apply eqb_eq.
-  - inversion tlt. tl_reflect H4.
-    specialize (IHsub ann_b b' tlt0). simpl in IHsub.
-    simpl. apply IHsub.
-  - inversion tlt.
-    tl_reflect H1. tl_reflect H4.
-    specialize (IHsub1 ann_t1 t1' tlt0).
-    specialize (IHsub2 ann_t2 t2' tlt1).
-    simpl. destruct IHsub1, IHsub2. 
-    auto.
+  intros Γ x t. revert Γ.
+  induction t; intros Γ ann t' tlt;
+  inversion tlt; subst.
+  - constructor.
+  - apply tlt_rel. now apply find_index_weaken.
+  - apply inj_pair2 in H2. subst.
+    apply tlt_lambda. 
+    + assumption.
+    + now apply (IHt (x' :: Γ)).
+  - apply inj_pair2 in H2. subst. 
+    apply tlt_app.
+    + apply IHt1; assumption.
+    + apply IHt2; assumption.
 Qed.
 
-Lemma tl_subst : forall Γ k x v b ann_v ann_b ann_t v' b',
-  nth_error Γ k = Some x ->
+Lemma weaken_ctx_many : forall Γ1 Γ2 t ann t',
+  translatesTo remap_env Γ1 t ann t' ->
+  translatesTo remap_env (Γ1 ++ Γ2) t ann t'.
+Proof.
+  intros Γ1 Γ2 t. revert Γ1. induction t;
+  intros Γ1 ann t' tlt_t; 
+  inversion tlt_t; subst.
+  - constructor.
+  - apply tlt_rel. now apply find_index_weaken.
+  - apply inj_pair2 in H2. subst.
+    apply tlt_lambda. 
+    + assumption.
+    + now apply (IHt (x' :: Γ1)).
+  - apply inj_pair2 in H2. subst.
+    apply tlt_app.
+    + apply IHt1; assumption.
+    + apply IHt2; assumption.
+Qed.
+
+Lemma strengthen_shadowed_ctx : forall Γ x b ann_b b',
+  In x Γ ->
+  translatesTo remap_env (Γ ++ [x]) b ann_b b' ->
+  translatesTo remap_env Γ b ann_b b'.
+Proof.
+  intros Γ x b. revert Γ. induction b;
+  intros Γ ann_b b' Hin tlt; inversion tlt; subst.
+  - constructor.
+  - apply tlt_rel.
+    unfold find_index_string in H1.
+    destruct_str_eq x x0.
+    + subst. now rewrite find_index_app1 in H1.
+    + rewrite find_index_app1 in H1; auto.
+      now eapply find_index_not_outer.
+  - apply inj_pair2 in H2. subst.
+    apply tlt_lambda. 
+    + assumption.
+    + apply IHb.
+      * now right. 
+      * assumption.
+  - apply inj_pair2 in H2. subst.
+    apply tlt_app.
+    + apply IHb1; assumption.
+    + apply IHb2; assumption.
+Qed.
+
+Definition annot_csubst {v} (ann_v : annots box_type v) :
+  forall k {b} (ann_b : annots box_type b), annots box_type (csubst v k b).
+Proof.
+  fix f 2.
+  intros k t ann_b.
+  destruct t eqn:Et; cbn in *; try exact ann_b.
+  - destruct (_ ?= _).
+    * exact ann_v.
+    * exact ann_b.
+    * exact ann_b.
+  - refine (ann_b.1, bigprod_map _ ann_b.2).
+    apply f.
+  - exact (ann_b.1, f _ _ ann_b.2).
+  - exact (ann_b.1, (f _ _ ann_b.2.1, f _ _ ann_b.2.2)).
+  - exact (ann_b.1, (f _ _ ann_b.2.1, f _ _ ann_b.2.2)).
+  - refine (ann_b.1, (f _ _ ann_b.2.1, bigprod_map _ ann_b.2.2)).
+    intros.
+    exact (f _ _ X).
+  - exact (ann_b.1, f _ _ ann_b.2).
+  - refine (ann_b.1, bigprod_map _ ann_b.2).
+    intros.
+    exact (f _ _ X).
+  - refine (ann_b.1, bigprod_map _ ann_b.2).
+    intros.
+    exact (f _ _ X).
+Defined.
+
+Lemma csubst_shadowed : forall Γ x b ann_b b' v ann_v,
+  In x Γ ->
+  translatesTo remap_env (Γ ++ [x]) b ann_b b' ->
+  translatesTo remap_env (Γ ++ [x]) (csubst v (List.length Γ) b) (annot_csubst ann_v (List.length Γ) ann_b) b'.
+Proof.
+  intros Γ x b. revert Γ. induction b; 
+  intros Γ ann_b b' v ann_v Hin tlt; inversion tlt.
+  - constructor.
+  - simpl. unfold find_index_string in H1.
+    destruct (#|Γ| ?= n) eqn:Hc.
+    + apply Nat.compare_eq_iff in Hc as Hl.
+      subst. apply find_index_outer in H1 as Hx.
+      subst x. now apply find_index_outer_not_In in H1.
+    + apply find_index_Some_length in H1 as Hl.
+      apply Nat.compare_lt_iff in Hc.
+      rewrite last_length in Hl. lia.
+    + now apply tlt_rel.
+  - apply inj_pair2 in H2. subst.
+    specialize (IHb (x' :: Γ) ann_b0 b'0 v).
+    simpl in *. apply tlt_lambda; auto.
+  - apply inj_pair2 in H2. subst. 
+    simpl. apply tlt_app.
+    + apply IHb1; auto.
+    + apply IHb2; auto.
+Qed.
+
+Lemma csubst_correct : forall Γ x v b ann_v ann_b v' b',
+  ~ In x Γ ->
   translatesTo remap_env nil v ann_v v' ->
   translatesTo remap_env (Γ ++ [x]) b ann_b b' ->
-  translatesTo remap_env Γ (csubst v k b) ann_t (BigStepPIR.subst (bs_to_s x) v' b').
+  translatesTo remap_env Γ (csubst v (List.length Γ) b)
+  (annot_csubst ann_v (List.length Γ) ann_b)
+  (BigStepPIR.subst x v' b').
 Proof.
-  intros Γ k x v b ann_v ann_b ann_t v' b'. revert Γ k ann_t b'.
-  induction b; intros Γ k' ann_t b' inCtx tlt_v tlt_b; inversion tlt_b.
-  - simpl. apply tlt_tt.
-  - simpl in *. admit.
-  - destruct ann_t as [ty ann_sb].
-    (* lambda case, annotations need to have the right form *)
-    admit.
-  - simpl in *. subst.
-    destruct ann_t as [t_ty [ann_st1 ann_st2]].
-    specialize (IHb1 ann_t1 Γ k' ann_st1 t1' inCtx tlt_v H1).
-    specialize (IHb2 ann_t2 Γ k' ann_st2 t2' inCtx tlt_v H4).
-    apply (tlt_app remap_env Γ). apply IHb1. apply IHb2.
-Admitted.
+  intros Γ x v b. revert Γ. induction b;
+  intros Γ ann_v ann_b v' b' HnIn tlt_v tlt_b;
+  inversion tlt_b; subst.
+  - constructor.
+  - destruct_str_eq x x0; subst.
+    + apply find_index_outer_length in H1 as Hl; auto.
+      symmetry in Hl. apply Nat.compare_eq_iff in Hl.
+      simpl in *. rewrite eqb_refl, Hl.
+      now eapply weaken_ctx_many in tlt_v.
+    + apply find_index_not_outer in H1 as Hin; auto.
+      apply find_index_not_outer_length in H1 as Hl; auto.
+      unfold find_index_string in H1.
+      rewrite find_index_app1 in H1; auto.
+      simpl in *. destruct (#|Γ| ?= n) eqn:Hc.
+      * now apply Nat.compare_eq_iff, Nat.eqb_eq in Hc.
+      * apply find_index_Some_length in H1 as Hn.
+        now apply Nat.compare_lt_iff in Hc.
+      * rewrite Heqb. now apply tlt_rel.
+  - apply inj_pair2 in H2. subst.
+    simpl. destruct_str_eq x x'.
+    + apply tlt_lambda. 
+      * assumption.
+      * subst x'. assert (Hin : In x (x::Γ)) by now left.
+        specialize (csubst_shadowed (x :: Γ) x b ann_b0 b'0 v ann_v Hin H4).
+        intros. simpl in H.
+        specialize (strengthen_shadowed_ctx (x :: Γ) x (csubst v (S #|Γ|) b) (annot_csubst ann_v (S #|Γ|) ann_b0) b'0 Hin H) as Hctx'.
+        apply Hctx'.
+    + apply tlt_lambda.
+      * assumption.
+      * apply IHb; auto. now apply not_in_cons.
+  - apply inj_pair2 in H2. subst.
+    specialize (IHb1 Γ ann_v ann_t1 v' t1' HnIn tlt_v H1).
+    specialize (IHb2 Γ ann_v ann_t2 v' t2' HnIn tlt_v H4).
+    now apply tlt_app.
+Qed.
 
-Theorem stlc_correct : forall Γ 
+Theorem stlc_correct : forall
   t (ann_t : annots box_type t) t'
   v (ann_v : annots box_type v),
   [] e⊢ t ⇓ v ->
-  InSubset Γ t ->
-  InSubset Γ v ->
-  translatesTo remap_env Γ t ann_t t' ->
+  InSubset [] t ->
+  InSubset [] v ->
+  translate_term remap_env [] t ann_t = Some t' ->
   exists ann_v v' k,
-    translatesTo remap_env Γ v ann_v v' /\
+    translatesTo remap_env [] v ann_v v' /\
     eval t' v' k.
 Proof with (eauto using eval).
-  intros Γ t ann_t t' v ann_v ev. revert t'.
-  induction ev; intros t'' sub_t sub_v tlt_t;
-  inversion sub_t.
+  intros t ann_t t' v ann_v ev sub_t sub_v tlt.
+  apply translate_reflect in tlt; try apply NoDup_nil. 
+  revert t' tlt; induction ev; 
+  intros t'' tlt; inversion sub_t.
   - admit. (* nonsensible case right now *)
-  - (* apply, the sensible case which requires subst-lemma *) admit.
-  - (* mkApps case *) subst. invs tlt_t. admit.
+  - (* apply case *) admit.
+  - (* mkApps case *) subst. invs tlt. admit.
   - (* fix case *) subst. inversion sub_v. 
     apply mkApps_in_subset in H3 as [Hcontra _].
     inversion Hcontra.
-  - (* fix case *) inversion tlt_t. subst. admit.
-  - (* mkApps constr case *) subst. inversion tlt_t. subst.
+  - (* fix case *) inversion tlt. subst. admit.
+  - (* mkApps constr case *) subst. inversion tlt. subst.
     admit.
   - (* Atoms applied to values *) admit.
   (* Atoms *)
-  - subst. inversion tlt_t. exists ann. exists t''.
-    subst. eexists. split. apply tlt_tt. apply E_Constant. eauto.
+  - subst. inversion tlt. exists ann. exists t''.
+    subst. eexists. split. 
+    + apply tlt_tt. 
+    + apply E_Constant. eauto.
   - subst. inversion i.
-  - subst. exists ann_t. exists t''. inversion tlt_t. 
-    subst. eexists. split. apply tlt_t. apply E_LamAbs. eauto.
+  - subst. exists ann_t. exists t''. inversion tlt. 
+    subst. eexists. split. 
+    + apply tlt. 
+    + apply E_LamAbs. eauto.
 Admitted.
