theories/Subset.v
@@ -6,15 +6,15 @@ From VTL Require Import PIR BigStepPIR Translation Utils.
 
 Existing Instance EWcbvEval.default_wcbv_flags.
 
-From Coq Require Strings.String Lia.
+From Coq Require Import Strings.String Lia.
 
-Inductive InSubset (Γ : list bs) : EAst.term -> Prop :=
+Inductive InSubset (Γ : list string) : EAst.term -> Prop :=
   | S_tBox : InSubset Γ tBox
   | S_tRel : forall n res,
-    nth_error Γ n = Some res ->
+    nth_error Γ n = Some res -> (* should this be find_index?*)
     InSubset Γ (tRel n)
-  | S_tLambda : forall x b,
-    InSubset (x :: Γ) b ->
+  | S_tLambda : forall x x' b,
+    InSubset (x' :: Γ) b ->
     InSubset Γ (tLambda (BasicAst.nNamed x) b)
   | S_tApp : forall f a,
     InSubset Γ f ->
@@ -38,17 +38,6 @@ Proof.
       * apply Hus. assumption.
 Qed.
 
-Lemma subset_closed : forall Γ t,
-  InSubset Γ t ->
-  closedn #|Γ| t.
-Proof.
-  intros Γ t' sub. induction sub.
-  - reflexivity.
-  - now apply nth_error_Some_length, Nat.ltb_lt in H.
-  - auto.
-  - simpl. auto.
-Qed.
-
 Lemma subset_weaken : forall Γ x t,
   InSubset Γ t ->
   InSubset (Γ ++ [x]) t.
@@ -58,8 +47,8 @@ Proof.
   - apply (S_tRel (Γ ++ [x]) n res). 
     apply nth_error_Some_length in H as Hl.
     rewrite (nth_error_app1 Γ [x] Hl). assumption.
-  - constructor. apply IHsub.
-  - constructor; assumption.
+  - eapply S_tLambda. apply IHsub.
+  - apply S_tApp; assumption.
 Qed.
 
 Lemma subset_weaken_many : forall Γ1 Γ2 t,
@@ -71,11 +60,11 @@ Proof.
   - apply (S_tRel (Γ ++ Γ2) n res). 
     apply nth_error_Some_length in H as Hl.
     rewrite (nth_error_app1 Γ Γ2 Hl). assumption.
-  - constructor. apply IHsub.
-  - constructor; assumption.
+  - eapply S_tLambda. apply IHsub.
+  - apply S_tApp; assumption.
 Qed.
 
-Lemma csubst_in_sub' : forall (Γ1 Γ2 : list bs) x v b,
+Lemma csubst_in_sub' : forall (Γ1 Γ2 : list string) x v b,
   InSubset [] v ->
   InSubset (Γ1 ++ x :: Γ2) b ->
   InSubset (Γ1 ++ Γ2) (csubst v #|Γ1| b).
@@ -96,17 +85,17 @@ Proof.
       apply nth_error_Some_length, length_middle in H0.
       apply nth_error_Some_value in H0. destruct H0.
       apply (S_tRel (Γ1 ++ Γ2) n x0 H). assumption.
-  - simpl. constructor.
-    apply (IHb (x0 :: Γ1) x). apply H0.
+  - simpl. econstructor.
+    apply (IHb (x' :: Γ1) x). apply H0.
   - simpl. constructor. 
     apply (IHb1 Γ1 x); assumption.
     apply (IHb2 Γ1 x); assumption.
 Qed.
 
-Lemma csubst_in_sub : forall (Γ : list bs) x v b,
+Lemma csubst_in_sub : forall (Γ : list string) x v b,
   InSubset [] v ->
   InSubset (Γ ++ [x]) b ->
-  InSubset (Γ) (csubst v #|Γ| b).
+  InSubset Γ (csubst v #|Γ| b).
 Proof.
   intros. assert (forall t, InSubset Γ t = InSubset (Γ ++ []) t) by (rewrite app_nil_r; reflexivity).
   rewrite H1. eapply (csubst_in_sub' Γ [] x v b); assumption.
@@ -133,3 +122,14 @@ Proof.
   - assumption.
   - assumption.
 Admitted.
+
+Lemma tlt_in_sub : forall TT Γ t ann t',
+  translatesTo TT Γ t ann t' ->
+  InSubset Γ t.
+Proof.
+  intros. induction H; subst.
+  - constructor.
+  - econstructor. now apply find_index_to_nth_error in H.
+  - now eapply S_tLambda.
+  - now apply S_tApp.
+Qed.
