theories/Translation.v
@@ -9,8 +9,6 @@ From VTL Require Import Env PIR Utils.
 
 From Coq Require Import String BinInt List.
 
-Local Open Scope string_scope.
-
 Import Kernames ListNotations.
 Import MCMonadNotation.
 Import BasicAst EAst.
@@ -35,9 +33,6 @@ Definition remap_fun (kn : kername) (df : PIR.DefaultFun) :=
 Section translate.
 
 Context (TT : env PIR.ty).
-(* TODO: extend with context to get fresh variable names *)
-
-(* Print find_index_bs. *)
 
 Definition translate_ty : box_type -> option PIR.ty :=
   fix go (ty : box_type) :=
@@ -51,114 +46,103 @@ Definition translate_ty : box_type -> option PIR.ty :=
   | _ => None
   end.
 
-Fixpoint translate_term (ctx : list bs) (t : term) 
+Fixpoint translate_term (Γ : list string) (t : term) 
                         {struct t} : annots box_type t -> option PIR.term :=
   match t return annots box_type t -> option PIR.term with
   | tBox => fun b_ty => Some (PIR.Constant (ValueOf DefaultUniUnit tt)) (* temporary constant *)
   | tRel n => fun b_ty =>
-    match nth_error ctx n with
+    match nth_error Γ n with
     | Some id => Some (PIR.Var id)
     | None => None
     end
   | tLambda (nNamed x) t => fun '(ty, t_ty) =>
       match ty with
       | TArr a _ =>
+        let x' := gen_fresh (bs_to_s x) Γ in
         a' <- translate_ty a ;;
-        t' <- translate_term (x :: ctx) t t_ty ;;
-        Some (LamAbs x a' t')
+        t' <- translate_term (x' :: Γ) t t_ty ;;
+        Some (LamAbs x' a' t')
       | _ => None
       end
   | tApp s t => fun '(_, (s_ty, t_ty)) =>
-    s' <- translate_term ctx s s_ty ;;
-    t' <- translate_term ctx t t_ty ;;
+    s' <- translate_term Γ s s_ty ;;
+    t' <- translate_term Γ t t_ty ;;
     Some (PIR.Apply s' t')
   | _ => fun _ => None
   end.
 
 Inductive translatesTypeTo : box_type -> PIR.ty -> Prop :=
-  | tlty_tt  : translatesTypeTo TBox (PIR.Ty_Builtin DefaultUniUnit)
+  | tlty_tt : translatesTypeTo TBox (PIR.Ty_Builtin DefaultUniUnit)
   | tlty_fun : forall ty1 ty2 ty1' ty2',
       translatesTypeTo ty1 ty1' ->
       translatesTypeTo ty2 ty2' ->
       translatesTypeTo (TArr ty1 ty2) (PIR.Ty_Fun ty1' ty2')
-  | tlty_kn  : forall kn ty',
+  | tlty_kn : forall kn ty',
       lookup TT (string_of_kername kn) = Some ty' ->
       translatesTypeTo (TConst kn) ty'.
 
-Inductive translatesTo (ctx : list bs) : forall (t : term),
+Inductive translatesTo (Γ : list string) : forall (t : term),
   annots box_type t -> PIR.term -> Prop :=
-  | tlt_tt : forall ann, translatesTo ctx tBox ann (Constant (ValueOf DefaultUniUnit tt))
-  | tlt_rel : forall n x ann, (* look at rel ordering *)
-      nth_error ctx n = Some x ->
-      translatesTo ctx (tRel n) ann (Var x)
-  | tlt_lambda : forall x ty1 ty2 b ann_b ty1' b',
+  | tlt_tt : forall ann, translatesTo Γ tBox ann (Constant (ValueOf DefaultUniUnit tt))
+  | tlt_rel : forall n x ann,
+      find_index_string Γ x = Some n ->
+      translatesTo Γ (tRel n) ann (Var x)
+  | tlt_lambda : forall x x' ty1 ty2 b ann_b ty1' b',
       translatesTypeTo ty1 ty1' ->
-      translatesTo (x :: ctx) b ann_b b' ->
-      translatesTo ctx (tLambda (nNamed x) b) ((TArr ty1 ty2), ann_b) (LamAbs x ty1' b')
+      translatesTo (x' :: Γ) b ann_b b' ->
+      translatesTo Γ (tLambda (nNamed x) b) ((TArr ty1 ty2), ann_b) (LamAbs x' ty1' b')
   | tlt_app : forall t1 t2 t1' t2' ann_t1 ann_t2 ty,
-      translatesTo ctx t1 ann_t1 t1' ->
-      translatesTo ctx t2 ann_t2 t2' ->
-      translatesTo ctx (tApp t1 t2) (ty, (ann_t1, ann_t2)) (PIR.Apply t1' t2').
+      translatesTo Γ t1 ann_t1 t1' ->
+      translatesTo Γ t2 ann_t2 t2' ->
+      translatesTo Γ (tApp t1 t2) (ty, (ann_t1, ann_t2)) (PIR.Apply t1' t2').
 
 Theorem translate_type_reflect : forall ty ty',
-  translate_ty ty = Some ty' <-> translatesTypeTo ty ty'.
+  translate_ty ty = Some ty' -> translatesTypeTo ty ty'.
 Proof.
-  intros ty ty'; split.
-  - revert ty'. induction ty; try discriminate; intros ty' tl_ty.
-    + inversion tl_ty. apply tlty_tt. 
-    + inversion tl_ty as [Hty].
-      destruct (translate_ty ty1) as [ty1'|]; try discriminate.
-      destruct (translate_ty ty2) as [ty2'|]; try discriminate.
+  intros ty ty'. revert ty'. induction ty; try discriminate; 
+  intros ty' tl_ty; inversion tl_ty.
+    + apply tlty_tt.
+    + destruct (translate_ty ty1) as [ty1'|]; [|discriminate].
+      destruct (translate_ty ty2) as [ty2'|]; [|discriminate].
       specialize (IHty1 ty1' eq_refl).
       specialize (IHty2 ty2' eq_refl).
-      inversion Hty as [Hty'].
-      apply (tlty_fun ty1 ty2 ty1' ty2' IHty1 IHty2).
-    + inversion tl_ty as [Hl].
-      apply tlty_kn. apply Hl.
-  - intros tl_ty. induction tl_ty.
-    + auto.
-    + simpl. rewrite IHtl_ty1, IHtl_ty2. reflexivity.
-    + auto.
+      inversion H0 as [Hty'].
+      now eapply tlty_fun.
+    + now apply tlty_kn.
 Qed.
 
-Theorem translate_reflect : forall ctx t t' (ann : annots box_type t),
-  translate_term ctx t ann = Some t' <-> translatesTo ctx t ann t'.
+Theorem translate_reflect : forall Γ t t' (ann : annots box_type t),
+  NoDup Γ ->
+  translate_term Γ t ann = Some t' -> translatesTo Γ t ann t'.
 Proof.
-  split.
-  - revert ctx t'. induction t; try discriminate; intros ctx t' tl_t.
-    + inversion tl_t. apply tlt_tt.
-    + inversion tl_t as [Ht].
-      destruct (nth_error ctx n) eqn:El; try discriminate.
-      inversion Ht as [Ht'].
-      apply tlt_rel. apply El.
-    + inversion tl_t as [Ht]. destruct na; try discriminate.
+  intros Γ t. revert Γ. induction t; try discriminate; 
+  intros Γ t' ann nodup tl_t; inversion tl_t as [Ht].
+    + apply tlt_tt.
+    + destruct (nth_error Γ n) eqn:El; [|discriminate].
+      inversion Ht as [Ht']. apply tlt_rel. 
+      now apply nth_error_to_find_index in El. 
+    + destruct na; try discriminate.
       destruct ann as [[] ann_b]; try discriminate.
-      destruct (translate_ty dom) as [ty1'|] eqn:tl_ty; try discriminate.
-      destruct (translate_term (i :: ctx) t ann_b) as [b'|] eqn:tl_b; try discriminate.
-      inversion Ht as [Ht']. subst.
-      specialize (IHt ann_b (i :: ctx) b' tl_b).
+      destruct (translate_ty dom) as [ty1'|] eqn:tl_ty; [|discriminate].
+      destruct (translate_term (gen_fresh i Γ :: Γ) t ann_b) as [b'|] eqn:tl_b; [|discriminate].
+      inversion Ht as [Ht']. assert (Hnodup' : NoDup (gen_fresh i Γ :: Γ)).
+      apply NoDup_cons. apply gen_fresh_fresh. assumption.
+      specialize (IHt (gen_fresh i Γ :: Γ) b' ann_b Hnodup' tl_b).
       apply (translate_type_reflect dom ty1') in tl_ty.
-      apply (tlt_lambda ctx i dom codom t ann_b ty1' b' tl_ty IHt).
-    + inversion tl_t as [Ht].
-      destruct ann as [ty [ann_t1 ann_t2]].
-      destruct (translate_term ctx t1 ann_t1) as [t1'|] eqn:tl_t1; try discriminate.
-      destruct (translate_term ctx t2 ann_t2) as [t2'|] eqn:tl_t2; try discriminate.
+      now apply tlt_lambda.
+    + destruct ann as [ty [ann_t1 ann_t2]].
+      destruct (translate_term Γ t1 ann_t1) as [t1'|] eqn:tl_t1; [|discriminate].
+      destruct (translate_term Γ t2 ann_t2) as [t2'|] eqn:tl_t2; [|discriminate].
       inversion Ht as [Ht'].
-      specialize (IHt1 ann_t1 ctx t1' tl_t1).
-      specialize (IHt2 ann_t2 ctx t2' tl_t2).
-      apply (tlt_app ctx t1 t2 t1' t2' ann_t1 ann_t2 ty IHt1 IHt2).
-  - intros tl_t. induction tl_t.
-    + auto.
-    + simpl. rewrite H. reflexivity.
-    + simpl. apply translate_type_reflect in H. rewrite H.
-      simpl. setoid_rewrite IHtl_t. reflexivity.
-    + simpl. rewrite IHtl_t1, IHtl_t2. reflexivity.
+      specialize (IHt1 Γ t1' ann_t1 nodup tl_t1).
+      specialize (IHt2 Γ t2' ann_t2 nodup tl_t2).
+      now apply tlt_app.
 Qed.
 
 End translate.
 
-Definition translate_unsafe ctx (t : term) (ann : annots box_type t) := 
-  with_default (PIR.Error (PIR.UNDEFINED "TranslationFailed")) (translate_term remap_env ctx t ann).
+Definition translate_unsafe Γ (t : term) (ann : annots box_type t) := 
+  with_default (PIR.Error (PIR.UNDEFINED "TranslationFailed")) (translate_term remap_env Γ t ann).
 
 (* Lambda Box T is the combination of an EAst term with a dependent tree of its types
   For now, we pass manual annotations until I set up a proper pipeline *)
